\documentclass[12pt,letterpaper]{article}
\author{Shawn Ma}
\date{\today}

\usepackage{amsmath}
\usepackage{amssymb}
\usepackage[letterspace=150]{microtype}
%\usepackage{asymptote}
\usepackage{geometry}
\usepackage{enumitem}
\usepackage{multicol}
\usepackage{setspace}
\usepackage{wasysym}
\usepackage{tcolorbox}

\geometry{left=2cm,right=2cm,top=1.5cm,bottom=1.5cm}
\begin{document}
%不要自动缩进
\setlength{\parindent}{0pt}
\setstretch{1.25}

\begin{enumerate}
    \item Compute the expressions below. Simplify the results. Use mixed numbers if possible.
    \begin{multicols}{2}
    \begin{enumerate}
        \item $\cfrac{1}{9}-\cfrac{5}{6}=$
        \item $\cfrac{11}{6}-\cfrac{5}{12}=$
        \item $\cfrac{11}{14}+\cfrac{7}{21}=$
        \item $2-\cfrac{8}{7}=$
        \item $\cfrac{12}{15}\times\cfrac{5}{8}=$
        \item $8\times\cfrac{9}{16}=$
        \item $\cfrac{5}{12}\times\cfrac{4}{10}=$
        \item $\cfrac{12}{7}\times\cfrac{14}{32}=$
        \item $15\times\cfrac{3}{10}=$
        \item $\cfrac{8}{15}\times\cfrac{10}{8}=$
        \item $\cfrac{4}{15}\div \cfrac{3}{8}=$
        \item $\cfrac{5}{12}\div 3=$
        \item $\cfrac{1}{12}\div \cfrac{1}{3}=$
        \item $7\div \cfrac{14}{5}=$
        \item $\cfrac{8}{18}\div \cfrac{16}{9}=$
        \item $\cfrac{3}{10}\div \cfrac{5}{8}=$
        \item $-4-2=$
        \item $-10+4=$
        \item $15+(-14)=$
        \item $-14+(-18)=$
        \item $-5-(-9)=$
        \item $-9+(-3)=$
        \item $9-(-3)=$
        \item $-2-(-19)=$
        \end{enumerate}
        \end{multicols}
        \pagebreak

        \item Simplify
        \begin{enumerate}
            \item $x+3y-5x-4y+7x=$
            \item $5x-9-(3x+4)=$
            \item $6x-4x+(2x-4x)+3=$
            \item $(4+2x)-(5x+2)=$
            \item $(-x+3)-(x+4)+(x-5)+(x+2)=$
            \item $43-2x-(x+3)=$
        \end{enumerate}
        \item Solve the equations
        \setstretch{4.5}
        \begin{enumerate}
            \item $3x=14-4x$
            \item $4x-7=15$
            \item $3x+1=-2x+6$
            \item $(4+3x)-(x-8)=19$
            \item $(x+3)+(x+4)=-1$
            \item $9x=17+2x$
        \end{enumerate}
\end{enumerate}
\end{document}
